Making progress

Term.thy
@@ -54,22 +54,19 @@ fun msg_of_term :: "(symbol, string) term \<Rightarrow> msg" where
 | "msg_of_term (Fun Sig_Symbol [k, m]) = Sig (msg_of_term k) (msg_of_term m)"
 | "msg_of_term _ = undefined"
 
-lemma wf_term_embed [simp]: "wf_term arity (embed msg)"
-  apply(induction msg)
-  by simp_all
+lemma wf_term_embed [simp]: "wf_term arity (embed m)"
+  by (induction m) simp_all
 
-lemma msg_of_term_embed [simp]: "msg_of_term (embed msg) = msg"
-  apply(induction msg)
-  by simp_all
+lemma msg_of_term_embed [simp]: "msg_of_term (embed m) = m"
+  by (induction m) simp_all
 
-lemma upper_bound_arity: "arity s = Suc (Suc (Suc x)) \<longleftrightarrow> False"
-  apply(cases s)
-  by simp_all
+lemma arity_upper_bound: "arity s = Suc (Suc (Suc x)) \<longleftrightarrow> False"
+  by (cases s) simp_all
 
 lemma embed_msg_of_term [simp]: "wf_term arity t \<Longrightarrow> embed (msg_of_term t) = t"
   apply(induction t rule: msg_of_term.induct)
-                      apply(simp_all add: upper_bound_arity)
-  apply(metis upper_bound_arity)
+                      apply(simp_all add: arity_upper_bound)
+  apply(metis arity_upper_bound)
   done
 
 lemma wf_subst_embed [simp]: "wf_subst arity (embed \<circ> \<sigma>)"
@@ -78,9 +75,10 @@ lemma wf_subst_embed [simp]: "wf_subst arity (embed \<circ> \<sigma>)"
 lemma msg_of_term_inject:
 "\<lbrakk> wf_term arity t1; wf_term arity t2 \<rbrakk>
 \<Longrightarrow> msg_of_term t1 = msg_of_term t2 \<longleftrightarrow> t1 = t2"
-  by (metis embed_msg_of_term)
+  using embed_msg_of_term by fastforce
 
 subsection \<open>(d)\<close>
+
 type_synonym msg_equation = "msg \<times> msg"
 type_synonym msg_equations = "msg_equation list"
 type_synonym symbol_subst = "string \<Rightarrow> (symbol, string) term"
@@ -92,8 +90,8 @@ definition msg_fv :: "msg \<Rightarrow> string set" where
 definition msg_sapply :: "msg_subst \<Rightarrow> msg \<Rightarrow> msg" (infixr "\<cdot>m" 67) where
   "msg_sapply \<sigma> m = msg_of_term ((embed \<circ> \<sigma>) \<cdot> (embed m))"
 
-definition msg_scomp :: "msg_subst \<Rightarrow> msg_subst \<Rightarrow> msg_subst" (infixl "\<circ>m" 55)
-  where "msg_scomp \<sigma> \<tau> = msg_of_term \<circ> ((embed \<circ> \<sigma>) \<circ>s (embed \<circ> \<tau>))"
+definition msg_scomp :: "msg_subst \<Rightarrow> msg_subst \<Rightarrow> msg_subst" (infixl "\<circ>m" 55) where 
+  "msg_scomp \<sigma> \<tau> = msg_of_term \<circ> ((embed \<circ> \<sigma>) \<circ>s (embed \<circ> \<tau>))"
 
 definition msg_fv_eq :: "msg_equation \<Rightarrow> string set" where
   "msg_fv_eq eq = (msg_fv (fst eq) \<union> msg_fv (snd eq))"
@@ -102,7 +100,7 @@ definition msg_fv_eqs :: "msg_equations \<Rightarrow> string set" where
   "msg_fv_eqs eqs = \<Union>(set (map msg_fv_eq eqs))"
 
 lemma fv_sapply: "msg_fv (\<sigma> \<cdot>m t) = fv ((embed \<circ> \<sigma>) \<cdot> (embed t))"
-  by (simp add: fv_sapply msg_fv_def msg_sapply_def wf_term_sapply)
+  by (simp add: msg_fv_def msg_sapply_def wf_term_sapply)
 
 definition msg_sdom :: "msg_subst \<Rightarrow> string set" where
   "msg_sdom \<sigma> = sdom (embed \<circ> \<sigma>)"
@@ -111,92 +109,87 @@ definition msg_svran :: "msg_subst \<Rightarrow> string set" where
   "msg_svran \<sigma> = svran (embed \<circ> \<sigma>)"
 
 lemma msg_sdom_var [simp]: "msg_sdom Variable = {}"
-  by(simp add: msg_sdom_def sdom_def)
+  by (simp add: msg_sdom_def sdom_def)
 
 lemma msg_svran_var [simp]: "msg_svran Variable = {}"
-  by(simp add: msg_svran_def svran_def sdom_def)
+  by (simp add: msg_svran_def svran_def sdom_def)
 
-lemma msg_var_ineq: "t \<noteq> Variable x \<Longrightarrow> embed t \<noteq> Var x"
-  by(metis msg_of_term.simps(1) msg_of_term_embed)
+lemma msg_not_var: "t \<noteq> Variable x \<longrightarrow> embed t \<noteq> Var x"
+  using msg_of_term_embed[of t] by force
 
 lemma msg_sdom_single_non_trivial [simp]: "t \<noteq> Variable x \<Longrightarrow> msg_sdom (Variable(x:=t)) = {x}"
-  by(simp add: msg_sdom_def sdom_def msg_var_ineq)
+  by (simp add: msg_sdom_def sdom_def msg_not_var)
 
 lemma msg_svran_single_non_trivial [simp]: "t \<noteq> Variable x \<Longrightarrow> msg_svran (Variable(x:=t)) = msg_fv t" 
-  by(auto simp add: msg_svran_def svran_def sdom_def msg_var_ineq msg_fv_def)
+  by (auto simp add: msg_svran_def svran_def sdom_def msg_not_var msg_fv_def)
 
 lemma msg_sdomI: "\<sigma> x \<noteq> Variable x \<Longrightarrow> x \<in> msg_sdom \<sigma>"
-  by(simp add: msg_sdom_def sdom_def msg_var_ineq)
+  by (simp add: msg_sdom_def sdom_def msg_not_var)
 
 lemma msg_fv_sapply_sdom_svran: "msg_fv (\<sigma> \<cdot>m t) \<subseteq> (msg_fv t - msg_sdom \<sigma>) \<union> msg_svran \<sigma>"
   unfolding msg_sdom_def msg_svran_def
   using svapply_svdom_svran msg_fv_def msg_sapply_def fv_sapply
-  by (simp; fastforce)
+  by (simp) fastforce
 
 lemma msg_sdom_scomp: "msg_sdom (\<sigma> \<circ>m \<tau>) \<subseteq> msg_sdom \<sigma> \<union> msg_sdom \<tau>"
   unfolding msg_sdom_def
   using sdom_scomp
   by (auto simp add: msg_scomp_def sdom_def scomp_sapply)
 
-(* TODO: Rewrite this proof *)
+lemma embed_msg_of_term_comp: "Term.embed \<circ> (msg_of_term \<circ> (Term.embed \<circ> \<sigma>) \<circ>s (Term.embed \<circ> \<tau>)) = (Term.embed \<circ> \<sigma>) \<circ>s (Term.embed \<circ> \<tau>)"
+  sorry
+
 lemma msg_svran_scomp: "msg_svran (\<sigma> \<circ>m \<tau>) \<subseteq> msg_svran \<sigma> \<union> msg_svran \<tau>"
   using svran_scomp[of "(embed \<circ> \<sigma>)" "(embed \<circ> \<tau>)"]
-  unfolding msg_svran_def svran_def sdom_def
-  apply (simp add: msg_scomp_def scomp_def fv_sapply)
-  apply (smt (verit, best) Collect_cong Sup.SUP_cong embed_msg_of_term wf_subst_embed wf_term_embed wf_term_sapply)
-  done
+  unfolding msg_svran_def msg_scomp_def
+  by (simp add: embed_msg_of_term_comp)
 
-(* TODO: Rewrite this proof *)
-lemma msg_scomp_distrib: 
-  "(\<sigma> \<circ>m \<tau>) \<cdot>m t = \<sigma> \<cdot>m (\<tau> \<cdot>m t)"
-  using sapply_scomp_distrib[of "(embed \<circ> \<sigma>)" "(embed \<circ> \<tau>)" "(embed t)"] 
-  apply (simp add: msg_scomp_def scomp_def msg_sapply_def)
-  apply (smt (verit, best) comp_apply embed_msg_of_term sapply_cong scomp_sapply wf_subst_embed wf_term_embed wf_term_sapply)
-  done
+lemma msg_scomp_distrib: "(\<sigma> \<circ>m \<tau>) \<cdot>m t = \<sigma> \<cdot>m (\<tau> \<cdot>m t)"
+  using sapply_scomp_distrib[of "(embed \<circ> \<sigma>)" "(embed \<circ> \<tau>)" "(embed t)"]
+  unfolding msg_scomp_def msg_sapply_def
+  by (simp add: embed_msg_of_term_comp wf_term_sapply)
 
 lemma msg_scomp_assoc: 
   "(\<sigma> \<circ>m \<tau>) \<circ>m \<upsilon> = \<sigma> \<circ>m (\<tau> \<circ>m \<upsilon>)"
-  using msg_scomp_distrib msg_sapply_def
+  using msg_scomp_distrib 
   unfolding msg_scomp_def scomp_def msg_sapply_def
   by fastforce
   
-lemma msg_var_sapply[simp]: "Variable \<cdot>m t = t"
+lemma msg_var_sapply [simp]: "Variable \<cdot>m t = t"
   using sapply_Var[of "embed t"]
   unfolding msg_sapply_def
   by (simp add: sapply_cong)
 
 lemma msg_var_sig: "Variable \<cdot>m (\<sigma> \<cdot>m x) = \<sigma> \<cdot>m x"
-  using msg_var_sapply
-  by simp
+  using msg_var_sapply by simp
 
-lemma msg_var_scomp[simp]: "\<sigma> \<circ>m Variable = \<sigma>"
+lemma msg_var_scomp [simp]: "\<sigma> \<circ>m Variable = \<sigma>"
   using scomp_Var[of "embed \<circ> \<sigma>"]
   unfolding msg_scomp_def comp_def
   by auto
 
 definition msg_unifies_eq :: "msg_subst \<Rightarrow> msg_equation \<Rightarrow> bool" where
-  "msg_unifies_eq \<sigma> pair = unifies_eq (embed \<circ> \<sigma>) (embed (fst pair), embed (snd pair))"
+  "msg_unifies_eq \<sigma> eq = unifies_eq (embed \<circ> \<sigma>) (embed (fst eq), embed (snd eq))"
 
-lemma msg_unifies_eq_alt: "msg_unifies_eq \<sigma> pair = (\<sigma> \<cdot>m fst(pair) = \<sigma> \<cdot>m snd(pair))"
-  unfolding msg_unifies_eq_def
-  by (simp add: wf_term_sapply msg_sapply_def msg_of_term_inject unifies_eq_def)
+lemma msg_unifies_eq_alt: "msg_unifies_eq \<sigma> eq = (\<sigma> \<cdot>m fst(eq) = \<sigma> \<cdot>m snd(eq))"
+  unfolding msg_unifies_eq_def unifies_eq_def
+  by (simp add: wf_term_sapply msg_sapply_def msg_of_term_inject)
 
 definition msg_unifies :: "msg_subst \<Rightarrow> msg_equations \<Rightarrow> bool" where
-  "msg_unifies \<sigma> pairs = unifies (embed \<circ> \<sigma>) (map (\<lambda>pair. map_prod embed embed pair) pairs)"
+  "msg_unifies \<sigma> eqs = unifies (embed \<circ> \<sigma>) (map (\<lambda>eq. map_prod embed embed eq) eqs)"
 
 (* remember: corresponding definition is a recursive function *)
-lemma msg_unifies_alt: "msg_unifies \<sigma> pairs = (\<forall>pair \<in> set pairs. msg_unifies_eq \<sigma> pair)"
-  unfolding msg_unifies_eq_def msg_unifies_def
-  apply (auto simp add: unifies_eq_def)
+lemma msg_unifies_alt: "msg_unifies \<sigma> eqs = (\<forall>eq \<in> set eqs. msg_unifies_eq \<sigma> eq)"
+  unfolding msg_unifies_def msg_unifies_eq_def 
   sorry
 
 definition msg_unify :: "msg_equations \<Rightarrow> msg_subst option" where
-  "msg_unify pairs = map_option ((\<circ>) msg_of_term) (unify (map (\<lambda>pair. map_prod embed embed pair) pairs))"
+  "msg_unify eqs = map_option ((\<circ>) msg_of_term) (unify (map (\<lambda>eq. map_prod embed embed eq) eqs))"
 
 definition msg_is_mgu :: "msg_subst \<Rightarrow> msg_equations \<Rightarrow> bool" where
-  "msg_is_mgu \<sigma> pairs = is_mgu (embed \<circ> \<sigma>) (map (\<lambda>pair. map_prod embed embed pair) pairs)"
+  "msg_is_mgu \<sigma> eqs = is_mgu (embed \<circ> \<sigma>) (map (\<lambda>eq. map_prod embed embed eq) eqs)"
 
-lemma msg_is_mgu_alt: "msg_is_mgu \<sigma> msg_pairs = (msg_unifies \<sigma> msg_pairs \<and> (\<forall>\<tau>. (msg_unifies \<tau> msg_pairs \<longrightarrow> (\<exists>\<tau>'. (\<tau> = \<tau>' \<circ>m \<sigma>)))))"
+lemma msg_is_mgu_alt: "msg_is_mgu \<sigma> eqs = (msg_unifies \<sigma> eqs \<and> (\<forall>\<tau>. (msg_unifies \<tau> eqs \<longrightarrow> (\<exists>\<tau>'. (\<tau> = \<tau>' \<circ>m \<sigma>)))))"
   apply(simp only: msg_is_mgu_def)
   apply(simp only: is_mgu_def)
   (* apply(simp only: unifies_eq_def)
